src/Language/PlutusIR/Semantics/SemanticEquivalence/CompatibilityLemmas.v
@@ -1,3 +1,4 @@
 Require Export PlutusCert.Language.PlutusIR.Semantics.SemanticEquivalence.CompatibilityLemmas.Apply.
 Require Export PlutusCert.Language.PlutusIR.Semantics.SemanticEquivalence.CompatibilityLemmas.Constant.
 Require Export PlutusCert.Language.PlutusIR.Semantics.SemanticEquivalence.CompatibilityLemmas.IWrap.
+Require Export PlutusCert.Language.PlutusIR.Semantics.SemanticEquivalence.CompatibilityLemmas.Unwrap.
