src/Language/PlutusIR/Semantics/SemanticEquivalence/CompatibilityLemmas/Unwrap.v
@@ -1,0 +1,294 @@
+Require Import PlutusCert.Language.PlutusIR.
+Import NamedTerm.
+Require Import PlutusCert.Language.PlutusIR.Semantics.Dynamic.
+Require Import PlutusCert.Language.PlutusIR.Semantics.Static.
+Require Import PlutusCert.Language.PlutusIR.Semantics.Static.Implementations.Named.
+Require Import PlutusCert.Language.PlutusIR.Semantics.Static.Implementations.Named.UniqueTypes.
+Require Import PlutusCert.Language.PlutusIR.Semantics.TypeSafety.Preservation.
+Require Import PlutusCert.Language.PlutusIR.Semantics.TypeSafety.SubstitutionPreservesTyping.
+Require Import PlutusCert.Language.PlutusIR.Semantics.SemanticEquivalence.Def.
+Require Import PlutusCert.Language.PlutusIR.Semantics.SemanticEquivalence.Monotonicity.
+Require Import PlutusCert.Language.PlutusIR.Semantics.SemanticEquivalence.ReductionInvariance.
+Require Import PlutusCert.Language.PlutusIR.Semantics.SemanticEquivalence.Termination.
+
+Require Import Arith.
+Require Import Coq.Logic.Decidable.
+
+Lemma inspect_eval__Unwrap_1 : forall e j e_f,
+    Unwrap e =[j]=> e_f ->
+    exists j_1 e_f1, e =[j_1]=> e_f1 /\ j_1 <= j.
+Proof.
+  intros.
+  inversion H. subst.
+  exists k0, (IWrap F T e_f). 
+  split; eauto.
+  rewrite plus_comm.
+  apply le_S.
+  apply le_n.
+Qed.
+
+Lemma helper0 : forall j,
+  j + 1 - j - 1 = 0.
+Proof. induction j; auto. Qed.
+
+Lemma inspect_eval__Unwrap_2 : forall e j e_f j_1 F T v_f11,
+    Unwrap e =[j]=> e_f ->
+    terminates_incl e j_1 (IWrap F T v_f11) j ->
+    j - j_1 - 1 = 0 /\ j = j_1 + 1 /\ e_f = v_f11.
+Proof.
+  intros.
+  inversion H. subst.
+  destruct H0.
+  assert (IWrap F0 T0 e_f = IWrap F T v_f11 /\ k0 = j_1) 
+    by (eapply eval__deterministic; eauto).
+  destruct H3. subst.
+  inversion H3. subst.
+  split; eauto using helper0.
+Qed.
+
+Lemma helper1 : forall k j,
+    j < k ->
+    0 < k.
+Proof.
+  intros.
+  inversion H.
+  - apply Nat.lt_0_succ.
+  - apply Nat.lt_0_succ.
+Qed.
+
+Lemma helper2 : forall k j,
+  j < k ->
+  k - j <= k.
+Proof.
+  induction 1.
+  - rewrite <- minus_Sn_m; auto.
+    rewrite Nat.sub_diag.
+    rewrite <- Nat.succ_le_mono.
+    apply Nat.le_0_l.
+  - rewrite <- minus_Sn_m; auto.
+    + rewrite <- Nat.succ_le_mono.
+      assumption.
+    + inversion H; subst.
+      * apply le_S. apply le_n.
+      * apply le_S.
+        rewrite Nat.succ_le_mono.
+        assumption.
+Qed.  
+
+Lemma helper3 : forall k j j_1,
+    j = j_1 + 1 ->
+    j_1 < k ->
+    k - j < k - j_1.
+Proof. Admitted.
+
+Lemma helper4 : forall k j,
+    j < k ->
+    0 < (k - j).
+Proof. Admitted.
+
+Lemma RC_compatibility_Unwrap : forall k F K T e e',
+    emptyContext |-* T : K ->
+    RC k (Ty_IFix F T) e e' ->
+    RC k (beta_reduce (unwrapIFix F K T)) (Unwrap e) (Unwrap e').
+Proof.
+  intros k F K T e e'.
+  intros Hkind_T H_RC.
+  remember H_RC as H_RC'. clear HeqH_RC'.
+
+  assert (Htyp : emptyContext |-+ (Unwrap e) : (beta_reduce (unwrapIFix F K T))). {
+    eapply T_Unwrap; eauto.
+    eapply RC_typable_empty_1; eauto.
+  } 
+  assert (Htyp' : emptyContext |-+ (Unwrap e') : (beta_reduce (unwrapIFix F K T))). {
+    eapply T_Unwrap; eauto.
+    eapply RC_typable_empty_2; eauto.
+  }
+
+  autorewrite with RC.
+
+  (* First part of the proof *)
+  split; auto. split; auto.
+
+  (* Second part of the proof *)
+
+  (** 
+      Consider arbitrary j, ef such that 
+      # j < k,
+      # Unwrap e -[j]-> e_f, and
+      # irred(e_f)
+  *)
+  intros j Hlt__j e_f ev__e.
+
+  (** 
+      Hence, by inspection of the operational semantics, it follows that there
+      exist j_1 and e_f1 such that
+      # e =[j_1]=> e_f1, 
+      # irred(e_f1) and
+      # j_1 <= j
+  *)
+  assert (temp: exists j_1 e_f1, e =[j_1]=> e_f1 /\ j_1 <= j) by eauto using inspect_eval__Unwrap_1.
+  destruct temp as [j_1 [e_f1 [Hev__e Hle__j_1]]].
+
+  (** 
+      Instantiate the second conjunct of H_RC with k. ... Instantiate this with 
+      j_1, e_f1. Note that
+      # j_1 < k, which follows from j_1 <= j < k,
+      # e =[j_1]=> e_f1, and
+      # irred(e_f1)
+  *)
+  assert (Hlt__j_1 : j_1 < k) by eauto using Nat.le_lt_trans. 
+
+  autorewrite with RC in H_RC.
+  destruct H_RC as [_ [_ H_RC]].
+  remember (H_RC j_1 Hlt__j_1 e_f1 Hev__e) as temp.
+  clear Heqtemp. clear H_RC. rename temp into H_RC.
+
+  (** 
+      Hence, there exists e'_f1 (and j'_1) such that
+      # e' =[j'_1]=> e'_f1, and
+      # (k - j_1, e_f1, e'_f1) \in RV[[Ty_IFix F T]]
+  *)
+  destruct H_RC as [e'_f1 [j'_1 [Hev__e1' H_RC]]].
+  assert (H_RV: RC (k - j_1) (Ty_IFix F T) e_f1 e'_f1). {
+    eapply RC_monotone.
+    - split.
+      + eapply eval_value. eapply eval_to_value. eauto.
+      + eapply helper1; eauto. 
+    - eapply eval_preserves_R; eauto.
+      split.
+      + eauto.
+      + eauto.
+    - apply helper2. assumption.
+  }
+
+  (**
+      Hence, 
+        e_f1 `equiv` IWrap F T v_f11, and
+        e'_f1 `equiv` IWrap F T v'_f11.
+  *)
+  assert (temp: exists v_f11, e_f1 = IWrap F T v_f11). {
+    apply skip. (* TODO *)
+  }
+  destruct temp as [v_f11 Heq1].
+  assert (temp: exists v'_f11, e'_f1 = IWrap F T v'_f11). {
+    apply skip. (* TODO *)
+  }
+  destruct temp as [v'_f11 Heq2].
+
+  (**
+      Note that
+        Unwrap e -[j_1]->
+        Unwrap e_f1 =
+        Unwrap (IWrap F T v_f11) -[1]->
+        v_f11 -[j - j1 - 1]->
+        e_f
+
+        Since v_f11 is a value, we have irred(v_f11).
+        Hence, j - j_1 -1 = 0 (and j = j_1 + 1) and e_f `equiv` v_f11.
+  *)
+  assert (temp: j - j_1 - 1 = 0 /\ j = j_1 + 1 /\ e_f = v_f11). {
+    subst. eapply inspect_eval__Unwrap_2; eauto. split; eauto.
+  }
+  destruct temp as [Heq3 [Heq4 Heq5]].
+
+  (**
+      Furthermore, note that
+        Unwrap e' -[j'_1]-> 
+        Unwrap e'_f1 =
+        Unwrap (IWrap F T v'_f11) -[1]->
+        v'_f11
+
+      Since v'_f11 is a value, we have irred(v'_f11).
+      Let e'f = v'_f11.
+  *)
+  exists (v'_f11). exists (j'_1 + 1).
+  
+  (** messy below *)
+  split. {
+    subst. eapply E_Unwrap; eauto.
+  }
+
+  assert (IWrap F T v_f11 = IWrap F T v_f11) by reflexivity.
+  assert (IWrap F T v'_f11 = IWrap F T v'_f11) by reflexivity.
+  assert (k - j < k - j_1) by (eapply helper3; eauto).
+  subst.
+  remember (H_RC _ _ H H0 _ H1 _ Hkind_T) as H_RC2.
+  clear HeqH_RC2.
+
+  assert (terminates_excl v_f11 0 v_f11 (k - (j_1 + 1))). {
+    split.
+    + eapply eval_value.
+      eapply eval_to_value.
+      eauto.
+    + eapply helper4; eauto.
+  }
+
+  destruct (beta_reduce (unwrapIFix F K T)) eqn:Hd.
+  - eapply RC_impossible_type in H_RC2; eauto.
+
+  - eapply RC_functional_extensionality in H_RC2; eauto.
+    destruct H_RC2 as [a [b [c H_RC2]]].
+    assert (a = v'_f11 /\ b = 0). {
+      
+      eapply eval__deterministic; eauto.
+      apply eval_value.
+      eapply eval_to_value; eauto.
+      eapply E_Unwrap. eauto.
+    }
+    destruct H3. subst.
+
+    intros.
+    eapply H_RC2; eauto.
+    rewrite <- minus_n_O.
+    auto.
+
+  - eapply RC_unwrap in H_RC2; eauto.
+    destruct H_RC2 as [a [b [c H_RC2]]].
+    assert (a = v'_f11 /\ b = 0). {
+      
+      eapply eval__deterministic; eauto.
+      apply eval_value.
+      eapply eval_to_value; eauto.
+      eapply E_Unwrap. eauto.
+    }
+    destruct H3. subst.
+
+    intros.
+    eapply H_RC2; eauto.
+    rewrite <- minus_n_O.
+    auto.
+
+  - eapply RC_instantiational_extensionality in H_RC2; eauto.
+    destruct H_RC2 as [a [b [c H_RC2]]].
+    assert (a = v'_f11 /\ b = 0). {
+      
+      eapply eval__deterministic; eauto.
+      apply eval_value.
+      eapply eval_to_value; eauto.
+      eapply E_Unwrap. eauto.
+    }
+    destruct H3. subst.
+
+    intros.
+    eapply H_RC2; eauto.
+    rewrite <- minus_n_O.
+    auto.
+
+  - eapply RC_syntactic_equality in H_RC2; eauto.
+    destruct H_RC2 as [a [b [c H_RC2]]].
+    assert (a = v'_f11 /\ b = 0). {
+      
+      eapply eval__deterministic; eauto.
+      apply eval_value.
+      eapply eval_to_value; eauto.
+      eapply E_Unwrap. eauto.
+    }
+    destruct H3. subst.
+
+    intros.
+    eapply H_RC2; eauto.
+
+  - eapply RC_impossible_type in H_RC2; eauto.
+
+  - eapply RC_impossible_type in H_RC2; eauto.
+Qed.
